Bumped fairneris model to be fairly terminating

fairneris/model_draft.v
@@ -1,5 +1,5 @@
 From trillium.prelude Require Export finitary quantifiers sigma classical_instances.
-From trillium.fairness Require Import fair_termination.
+From fairneris Require Import fairness.
 
 Import derived_laws_later.bi.
 
@@ -81,75 +81,310 @@ Lemma simple_live_spec_holds s ρ s' :
   simple_trans s ρ s' -> ρ ∈ simple_live_roles s.
 Proof. destruct s; inversion 1; try set_solver; destruct sent; set_solver. Qed.
 
+Definition network_fair_trace (mtr : trace simple_state simple_role) :=
+  ∀ n, pred_at mtr n (λ _ ℓ, ℓ ≠ Some Ndup ∧ ℓ ≠ Some Ndrop).
+
+Lemma network_fair_trace_after mtr mtr' k :
+  after k mtr = Some mtr' →
+  network_fair_trace mtr →
+  network_fair_trace mtr'.
+Proof.
+  rewrite /network_fair_trace.
+  intros Hafter Hfair.
+  intros n.
+  specialize (Hfair (k+n)).
+  rewrite pred_at_sum in Hfair.
+  rewrite Hafter in Hfair.
+  done.
+Qed.
+
 Definition simple_fair_model : FairModel.
 Proof.
   refine({|
             fmstate := simple_state;
             fmrole := simple_role;
             fmtrans := simple_trans;
+            fmfairness := network_fair_trace;
+            fmfairness_preserved := network_fair_trace_after;
             live_roles := simple_live_roles;
             fm_live_spec := simple_live_spec_holds;
           |}).
 Defined.
 
-(* (** Fair Model construction (currently does not work, as the config roles
-do not terminate) *) *)
+(** Fair Model construction (currently does not work, as the config roles
+do not terminate) *)
 
-(* Definition state_to_nat (s : simple_state) : nat := *)
-(*   match s with *)
-(*   | Start => 3 *)
-(*   | Sent _ => 2 *)
-(*   | Delivered _ _ => 1 *)
-(*   | Received _ _ => 0 *)
-(*   end. *)
+Definition state_to_nat (s : simple_state) : nat :=
+  match s with
+  | Start => 3
+  | Sent _ => 2
+  | Delivered _ _ => 1
+  | Received _ _ => 0
+  end.
 
-(* Definition simple_state_order (s1 s2 : simple_state) : Prop := *)
-(*   state_to_nat s1 ≤ state_to_nat s2. *)
+Definition simple_state_order (s1 s2 : simple_state) : Prop :=
+  state_to_nat s1 ≤ state_to_nat s2.
 
-(* Local Instance simple_state_order_preorder : PreOrder simple_state_order. *)
-(* Proof. *)
-(*   split. *)
-(*   - by intros []; constructor. *)
-(*   - intros [] [] []; rewrite /simple_state_order. *)
-(*     all: intros Hc12 Hc23; try by inversion Hc12. *)
-(*     all: rewrite /simple_state_order; try lia. *)
-(* Qed. *)
+Local Instance simple_state_order_preorder : PreOrder simple_state_order.
+Proof.
+  split.
+  - by intros []; constructor.
+  - intros [] [] []; rewrite /simple_state_order.
+    all: intros Hc12 Hc23; try by inversion Hc12.
+    all: rewrite /simple_state_order; try lia.
+Qed.
 
-(* Definition simple_decreasing_role (s : fmstate simple_fair_model) : *)
-(*   fmrole simple_fair_model := *)
-(*   match s with *)
-(*   | Start => A_role *)
-(*   | Sent _ => Ndeliver *)
-(*   | Delivered _ _ => B_role *)
-(*   | Received _ _ => Ndeliver    (* Why is this needed? *) *)
-(*   end. *)
+Definition simple_decreasing_role (s : fmstate simple_fair_model) :
+  fmrole simple_fair_model :=
+  match s with
+  | Start => A_role
+  | Sent _ => Ndeliver
+  | Delivered _ _ => B_role
+  | Received _ _ => Ndup    (* Why is this needed? *)
+  end.
 
-(* #[local] Program Instance simple_model_terminates : *)
-(*   FairTerminatingModel simple_fair_model := *)
-(*   {| *)
-(*     ftm_leq := simple_state_order; *)
-(*     ftm_decreasing_role := simple_decreasing_role; *)
-(*   |}. *)
-(* Next Obligation. *)
-(*   rewrite /simple_state_order. *)
-(*   intros []; repeat (constructor; intros [] []; simpl in *; try lia). *)
-(* Qed. *)
-(* Next Obligation. *)
-(*   rewrite /simple_state_order. *)
-(*   intros s [ρ' [s' Htrans]]=> /=. *)
-(*   split. *)
-(*   - destruct s; try set_solver. *)
-(*   - intros s'' Htrans'. simpl in *. *)
-(*     destruct s. *)
-(*     + inversion Htrans'. split; simpl; lia. *)
-(*     + inversion Htrans'. split; simpl; lia. *)
-(*     + inversion Htrans'. split; simpl; lia. *)
-(*     + inversion Htrans'. *)
-(* Qed. *)
-(* Next Obligation. *)
-(*   intros s s' ρ Htrans Hρ. by destruct s; inversion Htrans. *)
-(* Qed. *)
-(* Next Obligation. *)
-(*   rewrite /simple_state_order. *)
-(*   intros s1 ρ s2 Htrans. destruct s1; inversion Htrans; simpl; lia. *)
-(* Qed. *)
+(** Included redefinition of FairTerminatingModel here for now *)
+Class FairTerminatingModel (Mdl: FairModel) := {
+  ftm_leq: relation (Mdl.(fmstate));
+  ftm_order: PreOrder ftm_leq;
+  ftm_wf: wf (strict ftm_leq);
+
+  ftm_decreasing_role: fmstate Mdl → fmrole Mdl;
+  ftm_reachable_state: fmstate Mdl → Prop;
+
+  ftm_reachable: ∀ mtr, pred_at mtr 0 (λ ρ _, ftm_reachable_state ρ) →
+                        mtrace_valid mtr → mtrace_fair mtr →
+                        ∀ n, pred_at mtr n (λ _ _, True) →
+                             pred_at mtr n (λ δ _, ftm_reachable_state δ);
+  ftm_decr:
+    ∀ (s: fmstate Mdl), ftm_reachable_state s →
+                (∃ ρ' s', fmtrans _ s ρ' s') →
+                ftm_decreasing_role s ∈ live_roles _ s ∧
+                ∀ s', (fmtrans _ s (ftm_decreasing_role s) s' →
+                       (strict ftm_leq) s' s);
+  ftm_decreasing_role_preserved:
+    ∀ (s s': fmstate Mdl) ρ',
+      ftm_reachable_state s →
+      fmtrans _ s ρ' s' → ρ' ≠ ftm_decreasing_role s →
+      ftm_decreasing_role s = ftm_decreasing_role s';
+  ftm_notinc:
+    ∀ (s: fmstate Mdl) ρ s', ftm_reachable_state s → fmtrans _ s ρ s' → ftm_leq s' s;
+}.
+
+Arguments ftm_leq {_ _}.
+Arguments ftm_wf {_ _}.
+Arguments ftm_reachable_state {_ _}.
+Arguments ftm_reachable {_ _}.
+Arguments ftm_decr {_ _}.
+Arguments ftm_decreasing_role {_ _}.
+
+#[global] Existing Instance ftm_order.
+
+Notation ftm_lt := (strict ftm_leq).
+Local Infix "<" := ftm_lt.
+Local Infix "≤" := ftm_leq.
+
+Lemma ftm_trans' `{FairTerminatingModel Mdl} a b c:
+  a < b → b ≤ c → a < c.
+Proof.
+  intros [H1 H1'] H2.
+  (* TODO: Why do we need to extract this manually? *)
+  (* assert (EqDecision Mdl) by apply Mdl.(fmstate_eqdec). *)
+  destruct (decide (b = c)) as [->|Heq]; [done|].
+  split; [by etransitivity|].
+  intros H'. apply H1'.
+  by etransitivity.
+Qed.
+
+From Paco Require Import pacotac.
+
+Lemma fair_terminating_traces_terminate_rec `{FairTerminatingModel Mdl}
+      (s0: fmstate Mdl) (mtr: mtrace Mdl):
+  (trfirst mtr) ≤ s0 →
+  pred_at mtr 0 (λ ρ _, ftm_reachable_state ρ) →
+  mtrace_valid mtr →
+  mtrace_fair mtr →
+  terminating_trace mtr.
+Proof.
+  revert mtr. induction s0 as [s0 IH] using (well_founded_ind ftm_wf).
+  intros mtr Hleq Hinit Hval Hfair.
+  pose proof (ftm_reachable mtr Hinit Hval Hfair) as Hexcl.
+  destruct mtr as [|s ℓ mtr'] eqn:Heq; first by eexists 1.
+  destruct (ftm_decr (trfirst mtr)) as (Hlive & Htrdec).
+  { pose proof (Hexcl 0) as Hexcl0%pred_at_0; [|done]. by simplify_eq. }
+  { exists ℓ, (trfirst mtr'). punfold Hval. inversion Hval; subst; done. }
+  rewrite <- Heq in *. clear s ℓ Heq.
+  pose proof Hfair as [Hfair_scheduling _].
+  destruct (Hfair_scheduling (ftm_decreasing_role (trfirst mtr)) 0) as [n Hev];
+    first by rewrite /pred_at /=; destruct mtr.
+  clear Hfair_scheduling.
+  revert mtr Hexcl Hinit Hval Hleq Hfair Hlive IH Hev Htrdec. induction n as [| n IHn];
+    intros mtr Hexcl Hinit Hval Hleq Hfair Hlive IH Hev Htrdec.
+  - simpl in *. rewrite /pred_at /= in Hev.
+    destruct Hev as [Hev|Hev]; first by destruct mtr; done.
+    destruct mtr; first done. injection Hev => ->.
+    apply terminating_trace_cons.
+    eapply IH =>//; eauto.
+    + eapply ftm_trans' =>//. apply Htrdec.
+      punfold Hval. inversion Hval; simplify_eq; simpl in *; simplify_eq; done.
+    + apply (Hexcl 1). apply pred_at_S. by destruct mtr.
+    + punfold Hval. inversion Hval; simplify_eq.
+      destruct H4; done.
+    + destruct Hfair as [Hscheduling Hfair].
+      split.
+      * intros ρ. by eapply fair_model_trace_cons.
+      * eapply (fmfairness_preserved _ _ _ 1); [|apply Hfair]. done.
+  - simpl in *. destruct mtr; first (exists 1; done).
+    rewrite -> !pred_at_S in Hev.
+    punfold Hval; inversion Hval as [|??? Htrans Hval']; simplify_eq.
+    destruct Hval' as [Hval'|]; last done.
+    destruct (decide (ℓ = ftm_decreasing_role s)) as [-> | Hnoteq].
+    + apply terminating_trace_cons. eapply IH=>//; eauto.
+      eapply ftm_trans' =>//; apply Htrdec. simpl. destruct Hval; done.
+      * apply (Hexcl 1). apply pred_at_S. by destruct mtr.
+      * destruct Hfair as [Hscheduling Hfair].
+        split.
+        -- intros ρ. by eapply fair_model_trace_cons.
+        -- eapply (fmfairness_preserved _ _ _ 1); [|apply Hfair]. done.
+    + destruct mtr as [|s' ℓ' mtr''] eqn:Heq; first by eexists 2.
+      destruct (ftm_decr (trfirst mtr)) as (Hlive' & Htrdec').
+      { pose proof (Hexcl 1) as Hexcl0%pred_at_0; [|done]. by simplify_eq.}
+      { exists ℓ', (trfirst mtr''). punfold Hval'; inversion Hval'; subst; done. }
+      apply terminating_trace_cons. eapply IHn=>//; eauto.
+      * apply ftm_reachable; [|apply Hval'|].
+        -- apply (Hexcl 1). apply pred_at_S, pred_at_0. done.
+        -- split.
+           ++ intros ρ. eapply (fair_model_trace_after _ _ _ 1); [|apply Hfair]. done.
+           ++ eapply (fmfairness_preserved _ _ _ 1); [|apply Hfair]. done.
+      * apply (Hexcl 1). apply pred_at_S, pred_at_0. done.
+      * etransitivity; eauto. eapply ftm_notinc =>//.
+      * destruct Hfair as [Hscheduling Hfair].
+        split.
+       -- intros ρ. by eapply fair_model_trace_cons.
+       -- eapply (fmfairness_preserved _ _ _ 1); [|apply Hfair]. done.
+      * simplify_eq. eapply Hlive'.
+      * erewrite <- ftm_decreasing_role_preserved =>//.
+      * intros s'' Htrans''. eapply ftm_decr; eauto.
+        by pose proof (Hexcl 1) as Hexcl0%pred_at_0.
+Qed.
+
+Definition mtrace_fairly_terminating (mtr : mtrace simple_fair_model) :=
+  mtrace_valid mtr →
+  mtrace_fair mtr →
+  (* This needs to be strengthened to consider config steps *)
+  terminating_trace mtr.
+
+Theorem fair_terminating_traces_terminate `{FairTerminatingModel simple_fair_model} :
+  ∀ (mtrace : @mtrace simple_fair_model),
+    pred_at mtrace 0 (λ ρ _, ftm_reachable_state ρ) →
+    mtrace_fairly_terminating mtrace.
+Proof. intros ???[??]. eapply fair_terminating_traces_terminate_rec=>//. Qed.
+
+Definition simple_reachable_state s :=
+  match s with
+  | Sent 1 => True
+  | Sent n => False
+  | Delivered 0 0 => True
+  | Delivered n m => False
+  | Received 0 0 => True
+  | Received n m => False
+  | _ => True
+  end.
+
+Lemma mtrace_valid_after `{M : FairModel} (mtr mtr' : mtrace M) k :
+  after k mtr = Some mtr' → mtrace_valid mtr → mtrace_valid mtr'.
+Proof.
+  revert mtr mtr'.
+  induction k; intros mtr mtr' Hafter Hvalid.
+  { destruct mtr'; simpl in *; by simplify_eq. }
+  punfold Hvalid.
+  inversion Hvalid as [|??? Htrans Hval']; simplify_eq.
+  eapply IHk; [done|].
+  by inversion Hval'.
+Qed.
+
+#[local] Program Instance simple_model_terminates :
+  FairTerminatingModel simple_fair_model :=
+  {|
+    ftm_leq := simple_state_order;
+    ftm_decreasing_role := simple_decreasing_role;
+    ftm_reachable_state := simple_reachable_state;
+  |}.
+Next Obligation.
+  rewrite /simple_state_order.
+  intros []; repeat (constructor; intros [] []; simpl in *; try lia).
+Qed.
+Next Obligation.
+  intros mtr Hinit Hvalid [Hscheduling Hfair] n Hlen.
+  rewrite /pred_at in Hlen. rewrite /pred_at.
+  induction n; [done|].
+  destruct mtr; [done|].
+  assert (match after n (s -[ ℓ ]-> mtr) with
+        | None => False
+        | _ => True
+        end) as Hn.
+  { clear IHn. clear Hinit Hvalid Hscheduling Hfair. revert s mtr ℓ Hlen.
+    induction n; [done|]; intros s mtr ℓ Hlen.
+    simpl in *. destruct mtr; [done|].
+    simpl in *. apply IHn. done. }
+  assert (match after n (s -[ ℓ ]-> mtr) with
+          | Some ⟨ s ⟩ | Some (s -[ _ ]-> _) => simple_reachable_state s
+          | None => False
+          end) as IHn'.
+  { apply IHn. destruct (after n (s -[ ℓ ]-> mtr)); [|done]. destruct t; done. }
+  clear Hn IHn.
+  replace (S n) with (1 + n) by lia.
+  replace (S n) with (1 + n) in Hlen by lia.
+  rewrite after_sum.
+  rewrite after_sum in Hlen.
+  destruct (after n (s -[ ℓ ]-> mtr)) as [mtr'|] eqn:Heq; [|done].
+  destruct mtr' as [mtr''|mtr'' ℓ' mtr''']; [done|].
+  simpl in *.
+  assert (simple_trans mtr'' ℓ' (trfirst mtr''')).
+  { assert (mtrace_valid ((mtr'' -[ℓ']-> mtr'''):mtrace simple_fair_model)) as Hvalid'.
+    { by eapply mtrace_valid_after. }
+    punfold Hvalid'.
+    inversion Hvalid'.
+    simplify_eq.
+    apply H1. }
+  assert (network_fair_trace ((mtr'' -[ℓ']-> mtr'''):mtrace simple_fair_model)) as
+    Hfair'.
+  { by eapply network_fair_trace_after. }
+  inversion H; simplify_eq; try by inversion Hinit.
+  - rewrite /trfirst in H3. destruct mtr'''; by rewrite -H3.
+  - rewrite /trfirst in H3. destruct mtr'''; by rewrite -H3.
+  - rewrite /trfirst in H3. destruct mtr'''; by rewrite -H3.
+  - rewrite /network_fair_trace in Hfair.
+    specialize (Hfair' 0). by destruct Hfair' as [Hfair' ?].
+  - rewrite /network_fair_trace in Hfair.
+    specialize (Hfair' 0). by destruct Hfair' as [Hfair' ?].
+  - rewrite /trfirst in H3. destruct mtr'''; by rewrite -H3.
+  - rewrite /trfirst in H3. destruct mtr'''; by rewrite -H3.
+  - rewrite /network_fair_trace in Hfair.
+    specialize (Hfair' 0). by destruct Hfair' as [Hfair' ?].
+  - rewrite /trfirst in H3. destruct mtr'''; by rewrite -H3.
+  - rewrite /trfirst in H3. destruct mtr'''; by rewrite -H3.
+  - rewrite /trfirst in H3. destruct mtr'''; by rewrite -H3.
+  - rewrite /trfirst in H3. destruct mtr'''; by rewrite -H3.
+  - rewrite /trfirst in H3. destruct mtr'''; by rewrite -H3.
+Qed.
+Next Obligation.
+  rewrite /simple_state_order.
+  intros s Hexcl [ρ' [s' Htrans]]=> /=.
+  split.
+  - destruct s; try set_solver; destruct sent; try set_solver.
+    simpl in *. destruct delivered; try set_solver. inversion Htrans.
+  - intros s'' Htrans'. simpl in *.
+    destruct s.
+    + inversion Htrans'. split; simpl; lia.
+    + inversion Htrans'. split; simpl; lia.
+    + inversion Htrans'. split; simpl; lia.
+    + inversion Htrans'. simplify_eq. simpl in *. done.
+Qed.
+Next Obligation.
+  intros s s' ρ Hreachable Htrans Hρ. by destruct s; inversion Htrans.
+Qed.
+Next Obligation.
+  rewrite /simple_state_order.
+  intros s1 ρ s2 Hreachable Htrans. destruct s1; inversion Htrans; simpl; lia.
+Qed.
