fairneris/fairness.v
@@ -1,0 +1,181 @@
+From stdpp Require Import option.
+From Paco Require Import paco1 paco2 pacotac.
+From trillium.fairness Require Export inftraces.
+
+Record FairModel : Type := {
+  fmstate: Type;
+  fmstate_eqdec: EqDecision fmstate;
+  fmstate_inhabited: Inhabited fmstate;
+
+  fmrole: Type;
+  fmrole_eqdec: EqDecision fmrole;
+  fmrole_countable: Countable fmrole;
+  fmrole_inhabited: Inhabited fmrole;
+
+  fmtrans: fmstate → fmrole → fmstate → Prop;
+  fmfairness : trace fmstate fmrole → Prop;
+  fmfairness_preserved : ∀ mtr mtr' k, after k mtr = Some mtr' →
+                                       fmfairness mtr →
+                                       fmfairness mtr';
+
+  live_roles: fmstate → gset fmrole;
+  fm_live_spec: ∀ s ρ s', fmtrans s ρ s' → ρ ∈ live_roles s;
+
+}.
+
+#[global] Existing Instance fmstate_eqdec.
+#[global] Existing Instance fmstate_inhabited.
+#[global] Existing Instance fmrole_eqdec.
+#[global] Existing Instance fmrole_countable.
+#[global] Existing Instance fmrole_inhabited.
+
+Definition fair_model_to_model (FM : FairModel) : Model :=
+  {|
+    mstate := fmstate FM;
+    mlabel := fmrole FM;
+    mtrans := fmtrans FM;
+  |}.
+
+(* Basically, soundness of the logic and the lemmas above tell us that we have a program
+   trace and a model trace which are related by traces_match labels_math!
+
+   We now prove that this relation transports the properties we care about; the first
+   place of which is fairness.
+ *)
+
+(* Definition of fairness for both kinds of traces *)
+
+Definition extrace Λ := trace (cfg Λ) (ex_label Λ).
+
+Section exec_trace.
+  Context {Λ : language}.
+  Context `{EqDecision (locale Λ)}.
+
+  Definition locale_enabled (ζ : locale Λ) (c: cfg Λ) :=
+    ∃ e, from_locale c.1 ζ = Some e ∧ to_val e = None.
+
+  Definition fair_ex ζ (extr: extrace Λ): Prop :=
+    ∀ n, pred_at extr n (λ c _, locale_enabled ζ c) →
+         ∃ m, pred_at extr (n+m) (λ c _, ¬locale_enabled ζ c) ∨
+              pred_at extr (n+m) (λ _ otid, otid = Some (inl ζ)).
+
+  Definition config_enabled (ζ : config_label Λ) := True.
+
+  Definition fair_config_ex ζ (extr : extrace Λ) : Prop :=
+    ∀ n, pred_at extr n (λ c _, config_enabled ζ) →
+         ∃ m, pred_at extr (n+m) (λ c _, ¬config_enabled ζ) ∨
+              pred_at extr (n+m) (λ _ otid, otid = Some (inr ζ)).
+
+  Lemma fair_ex_after ζ tr tr' k:
+    after k tr = Some tr' →
+    fair_ex ζ tr → fair_ex ζ tr'.
+  Proof.
+    intros Haf Hf n Hp.
+    have Hh:= Hf (k+n).
+    have Hp': pred_at tr (k + n) (λ (c : cfg Λ) (_ : option (ex_label Λ)), locale_enabled ζ c).
+    { rewrite (pred_at_sum _ k) Haf /= //. }
+    have [m Hm] := Hh Hp'. exists m.
+    by rewrite <- Nat.add_assoc, !(pred_at_sum _ k), Haf in Hm.
+  Qed.
+
+  Lemma fair_ex_cons tid c tid' r:
+    fair_ex tid (c -[tid']-> r) → fair_ex tid r.
+  Proof. intros H. by eapply (fair_ex_after tid (c -[tid']-> r) r 1). Qed.
+
+  CoInductive extrace_valid: extrace Λ → Prop :=
+  | extrace_valid_singleton c: extrace_valid ⟨c⟩
+  | extrace_valid_cons c oζ tr:
+      locale_step c oζ (trfirst tr) →
+      extrace_valid tr →
+      extrace_valid (c -[oζ]-> tr).
+
+  Lemma to_trace_preserves_validity ex iex:
+    extrace_valid (to_trace (trace_last ex) iex) → valid_exec ex → valid_inf_exec ex iex.
+  Proof.
+    revert ex iex. cofix CH. intros ex iex Hexval Hval.
+    rewrite (trace_unfold_fold (to_trace _ _)) in Hexval.
+    destruct iex as [|[??] iex]; first by econstructor. cbn in Hexval.
+    inversion Hexval. simplify_eq.
+    econstructor; try done.
+    - by destruct iex as [|[??]?].
+    - apply CH; eauto. econstructor; try done. by destruct iex as [|[??]?].
+  Qed.
+
+  Lemma from_trace_preserves_validity (extr: extrace Λ) ex:
+    extrace_valid extr →
+    valid_exec ex →
+    trace_last ex = trfirst extr →
+    valid_inf_exec ex (from_trace extr).
+  Proof.
+    revert ex extr. cofix CH. intros ex extr Hexval Hval Heq.
+    rewrite (inflist_unfold_fold (from_trace extr)). destruct extr as [c|c tid tr]; cbn;
+     first by econstructor.
+    inversion Hexval; simplify_eq; econstructor; eauto. apply CH; eauto.
+      by econstructor.
+  Qed.
+
+  Lemma from_trace_preserves_validity_singleton (extr: extrace Λ):
+    extrace_valid extr →
+    valid_inf_exec (trace_singleton (trfirst extr)) (from_trace extr).
+  Proof.
+    intros ?. eapply from_trace_preserves_validity; eauto. econstructor.
+  Qed.
+
+End exec_trace.
+
+Definition mtrace (M:FairModel) := trace (M.(fmstate)) (M.(fmrole)).
+
+Section model_traces.
+  Context `{M: FairModel}.
+
+  Definition role_enabled_model ρ (s: M.(fmstate)) := ρ ∈ M.(live_roles) s.
+
+  Definition fair_model_trace ρ (mtr: mtrace M): Prop  :=
+    forall n, pred_at mtr n (λ δ _, role_enabled_model ρ δ) →
+         ∃ m, pred_at mtr (n+m) (λ δ _, ¬role_enabled_model ρ δ)
+              ∨ pred_at mtr (n+m) (λ _ ℓ, ℓ = Some ρ).
+
+  Lemma fair_model_trace_after ℓ tr tr' k:
+    after k tr = Some tr' →
+    fair_model_trace ℓ tr → fair_model_trace ℓ tr'.
+  Proof.
+    intros Haf Hf n Hp.
+    have Hh:= Hf (k+n).
+    have Hp': pred_at tr (k + n) (λ δ _, role_enabled_model ℓ δ).
+    { rewrite (pred_at_sum _ k) Haf /= //. }
+    have [m Hm] := Hh Hp'. exists m.
+    by rewrite <- Nat.add_assoc, !(pred_at_sum _ k), Haf in Hm.
+  Qed.
+
+  Lemma fair_model_trace_cons ℓ δ ℓ' r:
+    fair_model_trace ℓ (δ -[ℓ']-> r) → fair_model_trace ℓ r.
+  Proof. intros Hfm. by eapply (fair_model_trace_after ℓ _ r 1) =>//. Qed.
+
+  Lemma fair_model_trace_cons_forall δ ℓ' r:
+    (∀ ℓ, fair_model_trace ℓ (δ -[ℓ']-> r)) → (∀ ℓ, fair_model_trace ℓ r).
+  Proof. eauto using fair_model_trace_cons. Qed.
+
+  Definition fair_scheduling mtr := ∀ ρ, fair_model_trace ρ mtr.
+  Definition mtrace_fair mtr := fair_scheduling mtr ∧ M.(fmfairness) mtr.
+
+  Inductive mtrace_valid_ind (mtrace_valid_coind: mtrace M → Prop) :
+    mtrace M → Prop :=
+  | mtrace_valid_singleton δ: mtrace_valid_ind _ ⟨δ⟩
+  | mtrace_valid_cons δ ℓ tr:
+      fmtrans _ δ ℓ (trfirst tr) →
+      mtrace_valid_coind tr →
+      mtrace_valid_ind _ (δ -[ℓ]-> tr).
+  Definition mtrace_valid := paco1 mtrace_valid_ind bot1.
+
+  Lemma mtrace_valid_mono :
+    monotone1 mtrace_valid_ind.
+  Proof.
+    unfold monotone1. intros x0 r r' IN LE.
+    induction IN; try (econstructor; eauto; done).
+  Qed.
+  Hint Resolve mtrace_valid_mono : paco.
+
+End model_traces.
+
+Global Hint Resolve fair_model_trace_cons: core.
+Global Hint Resolve mtrace_valid_mono : paco.
